IOHist.fst
@@ -57,36 +57,3 @@ let rec iohist_interpretation #a
       let event : io_event = convert_call_to_event cmd args res in
       iohist_interpretation (fnc res) (event :: past_events) (gen_post p event)))
   end
-
-
-let rec fin_prefs #a
-  (m : io a) 
-  (past_events : events_trace) 
-  (traces : list events_trace) : Type0 = 
-  match m with
-  | Return x -> past_events `List.memP` traces
-  | Throw err -> past_events `List.memP` traces
-  | Cont t -> begin
-    match t with
-    | Call cmd args fnc -> (forall res. (
-      FStar.WellFounded.axiom1 fnc res;
-      let event : io_event = convert_call_to_event cmd args res in
-      fin_prefs (fnc res) (event :: past_events) traces))
-  end
-
-(* total *)
-(* reifiable *)
-(* reflectable *)
-(* new_effect { *)
-(*   IOHist : a:Type -> Effect *)
-(*   with  *)
-(*        repr       = io *)
-(*      ; return     = io_return *)
-(*      ; bind       = io_bind *)
-
-(*      ; wp_type    = iohist_wpty *)
-(*      ; return_wp  = iohist_return_wp *)
-(*      ; bind_wp    = iohist_bind_wp *)
-
-(*      ; interp     = iohist_interpretation *)
-(* } *)
