rsp.fst
@@ -1,0 +1,103 @@
+module Rsp
+
+open FStar.Tactics
+
+open Common
+open IOStHist
+open M4
+open Minterop
+
+type set_of_traces = events_trace -> Type0
+
+val included_in : set_of_traces -> set_of_traces -> Type0
+let included_in s1 s2 = forall t. s1 t ==>  s2 t
+
+let rec behavior #a
+  (m : io a) : set_of_traces =
+  match m with
+  | Return x -> fun t -> t == []
+  | Throw err -> fun t -> t == []
+  | Cont t -> begin
+    match t with
+    | Call cmd args fnc -> (fun t' -> 
+      (exists res t. (
+         FStar.WellFounded.axiom1 fnc res;
+         (behavior (fnc res) t) /\
+         t' == ((convert_call_to_event cmd args res)::t))))
+  end
+
+let included_in_trans #a #b #c () : Lemma (
+  forall (t1:io a) (t2:io b) (t3:io c). behavior t1 `included_in` behavior t2 /\ behavior t2 `included_in` behavior t3 ==>
+    behavior t1 `included_in` behavior t3) = ()
+
+let behavior_iost_to_io () : Lemma
+  (forall a tree. behavior (iost_to_io tree) `included_in` behavior tree) = admit ()
+
+// let interstinglemma #a (x: io a) : Lemma (
+//   let xx = M4?.reflect (fun _ -> x) <: M4wp a (fun p -> forall res. p res) in
+//   behavior (reify xx) (fun _ -> True) `include_in` behavior x) = ()
+
+let interstinglemma () : Lemma (forall a x.
+  let xx : unit -> M4 a = (fun () -> (M4?.reflect (fun _ -> x) <: M4wp a (fun p -> forall res. p res))) in
+  behavior (reify (xx ()) (fun _ -> True)) `included_in` behavior x) = ()
+    
+let pre_lemma #t1
+  (pre : t1 -> events_trace -> Type0)  {| checkable2 pre |}
+  (x : t1): Lemma (check2 #t1 #events_trace #pre x [] == true) = admit()
+
+// let export_lemma #t1 #t2
+//   {| d1:ml t1 |} {| d2:ml t2 |}
+//   (pre : t1 -> events_trace -> Type0)
+//   {| checkable2 pre |}
+//   (post : t1 -> events_trace -> maybe (events_trace * t2) -> events_trace -> Type0)
+//   (f:(x:t1 -> IOStHist t2 (pre x) (post x)))
+//   (x:t1)  : Lemma (
+//     let res' = reify ((_export_IOStHist_arrow_spec pre post f <: (t1 -> M4 t2)) x) (fun _ -> True) in
+//     let f' = reify (f x) (post x []) in
+//     check2 #t1 #events_trace #pre x [] == true ==>  behavior res' `included_in` behavior (f' [])
+//   ) =
+//   assume (behavior (iost_to_io (reify (f x) (post x []) [])) `included_in` behavior (reify (f x) (post x []) []));
+//   assert (
+//     check2 #t1 #events_trace #pre x [] == true ==>  behavior (reify ((_export_IOStHist_arrow_spec pre post f <: (t1 -> M4 t2)) x) (fun _ -> True)) `included_in` behavior (reify (f x) (post x []) []))
+//   by (
+//   let stst1 = implies_intro () in
+//   unfold_def (`included_in);
+//   let t = forall_intro () in
+//   unfold_def (`_export_IOStHist_arrow_spec);
+//   let tres = implies_intro () in
+//   binder_retype tres;
+    
+//     rewrite_eqs_from_context ();
+//   trefl ();
+//   dump "h"
+//   )
+
+
+let export_lemma #t1 #t2
+  {| d1:ml t1 |} {| d2:ml t2 |}
+  (pre : t1 -> events_trace -> Type0)
+  {| checkable2 pre |}
+  (post : t1 -> events_trace -> maybe (events_trace * t2) -> events_trace -> Type0)
+  (f:(x:t1 -> IOStHist t2 (pre x) (post x)))
+  (x:t1)  : Lemma (
+    let res' = reify ((_export_IOStHist_arrow_spec pre post f <: (t1 -> M4 t2)) x) (fun _ -> True) in
+    let f' = reify (f x) (post x []) in
+    check2 #t1 #events_trace #pre x [] == true ==>  behavior res' `included_in` behavior (f' [])
+  ) by (    
+  split ();
+  smt (); 
+  let pp = forall_intro () in
+  let myp = implies_intro () in
+  let pr = forall_intro () in
+  let asd = FStar.Tactics.Logic.instantiate (binder_to_term myp) (binder_to_term pr) in
+  mapply (binder_to_term asd);
+  let stst1 = implies_intro () in
+  unfold_def (`included_in);
+  let t = forall_intro () in
+  unfold_def (`_export_IOStHist_arrow_spec);
+  rewrite_eqs_from_context ();
+  dump "h";
+  tadmit ();
+  ()) = 
+  ()
+
